some lemmas about bounded predicate + incorporated in the proof; OK case done

src/C_strtoimax/VstProof/AbstractSpec.v
@@ -6,44 +6,39 @@ Import ListNotations.
 
 Section AbstractSpec.
 
-  Definition minus_char := Byte.repr 45.
-  Definition plus_char := Byte.repr 43.
-  Definition zero_char := Byte.repr 48.
-  Definition nine_char := Byte.repr 57.
+  Definition minus_char := 45.
+  Definition plus_char := 43.
+  Definition zero_char := 48.
+  Definition nine_char := 57.
 
   Definition is_digit (i : byte) : bool :=
-    ((zero_char <= i) && (i <= nine_char))%byte.
+    (zero_char <=? Byte.signed i) && (Byte.signed i <=? nine_char).
 
   Definition Z_of_char (b : byte) : Z :=
-    Byte.signed b - Byte.signed zero_char.
+    Byte.signed b - 48.
 
   Definition is_sign (b : byte) : bool :=
-    ((b == plus_char) || (b == minus_char))%byte.
-
-  Definition sign_of_char (b : byte) : Z :=
-    if (b == plus_char)%byte then 1
-    else if (b == minus_char)%byte then (- 1)
-         else 0.
+    (Byte.signed b =? plus_char) || (Byte.signed b =? minus_char).
 
   Definition bounded (n : Z) : bool :=
     andb (Int64.min_signed <=? n) (n <=? Int64.max_signed).
 
   Inductive asn_strtox_result_e :=
-  | ASN_STRTOX_ERROR_RANGE (* Input outside of supported numeric range *)
-  | ASN_STRTOX_ERROR_INVAL (* Invalid data encountered (e.g., "+-") *)
-  | ASN_STRTOX_EXPECT_MORE (* More data expected (e.g. "+") *)
-  | ASN_STRTOX_EXTRA_DATA  (* Conversion succeded, but the string has extra stuff *)
-  | ASN_STRTOX_OK.         (* Conversion succeded, number ends at (end) *)
+  | ERROR_RANGE (* Input outside of supported numeric range *)
+  | ERROR_INVAL (* Invalid data encountered (e.g., "+-") *)
+  | EXPECT_MORE (* More data expected (e.g. "+") *)
+  | EXTRA_DATA  (* Conversion succeded, but the string has extra stuff *)
+  | OK.         (* Conversion succeded, number ends at (end) *)
 
   (* C light outputs int *)
 
   Definition asn_strtox_result_e_to_int (s : asn_strtox_result_e) : int :=
     match s with
-    | ASN_STRTOX_ERROR_RANGE => Int.repr (-3)
-    | ASN_STRTOX_ERROR_INVAL => Int.repr (-2)
-    | ASN_STRTOX_EXPECT_MORE => Int.repr (-1)
-    | ASN_STRTOX_EXTRA_DATA => Int.repr 1
-    | ASN_STRTOX_OK => Int.repr 0
+    | ERROR_RANGE => Int.repr (-3)
+    | ERROR_INVAL => Int.repr (-2)
+    | EXPECT_MORE => Int.repr (-1)
+    | EXTRA_DATA => Int.repr 1
+    | OK => Int.repr 0
     end.
 
   Record Z_of_string_result :=
@@ -54,7 +49,7 @@ Section AbstractSpec.
   
   Fixpoint Z_of_string_loop (s : list byte) (v i : Z) := 
     match s with 
-    | [] => {| res := ASN_STRTOX_OK ; 
+    | [] => {| res := OK ; 
               value := v ; 
               index := i |}
     | c :: tl => 
@@ -62,10 +57,10 @@ Section AbstractSpec.
       then let v1 := v * 10 + (Z_of_char c) in 
            if bounded v1
            then Z_of_string_loop tl v1 (i + 1)
-           else {| res := ASN_STRTOX_ERROR_RANGE ;
+           else {| res := ERROR_RANGE ;
                    value := v1 ;
                    index := i ; |}      
-      else {| res := ASN_STRTOX_EXTRA_DATA ;
+      else {| res := EXTRA_DATA ;
               value := v ;
               index := i ; |}              
     end.
@@ -73,20 +68,20 @@ Section AbstractSpec.
 
   Definition Z_of_string (s : list byte) : Z_of_string_result := 
       match s with 
-      |  nil => {| res := ASN_STRTOX_ERROR_INVAL ; 
+      |  nil => {| res := ERROR_INVAL ; 
                   value := 0 ;
                   index := 0 ; |} 
       | [ch] => if is_sign ch 
-                then {| res := ASN_STRTOX_EXPECT_MORE ;
+                then {| res := EXPECT_MORE ;
                         value := 0 ;
                         index := 1 ; |} 
                 else Z_of_string_loop s 0 0
-      |  ch :: tl => let result := Z_of_string_loop tl 0 0 in
-                    if (ch == plus_char)%byte
+      |  ch :: tl => let result := Z_of_string_loop tl 0 1 in
+                    if (Byte.signed ch =? plus_char)
                     then result
-                    else if (ch == minus_char)%byte
-                         then {| res := ASN_STRTOX_OK ;
-                                 value := Z.opp (value result) ;
+                    else if (Byte.signed ch =? minus_char)
+                         then {| res := res result ;
+                                 value := -1 * (value result) ;
                                  index := index result ; |}
                          else Z_of_string_loop s 0 0
       end.
